Semantics/Seq_Semantics.thy
@@ -1,29 +1,22 @@
-theory Seq_Semantics imports "Gensyn_Semantics_TypeParam" "../Syntax/Syn_Seq"
+theory Seq_Semantics imports "Gensyn_Semantics" "../Syntax/Syn_Seq"
 begin
 
 locale Seq_Semantics_Sig =
   fixes xr :: "'xr itself"
   fixes ms :: "'mstate itself"
-  fixes seq_sem :: "'g \<Rightarrow> 'sq \<Rightarrow> 'mstate \<Rightarrow> 'mstate \<Rightarrow> bool"
+  fixes seq_sem :: "'sq \<Rightarrow> 'mstate \<Rightarrow> 'mstate \<Rightarrow> bool"
 
-inductive seq_nop :: "'g \<Rightarrow> 'sq \<Rightarrow> 'mstate \<Rightarrow> 'mstate \<Rightarrow> bool" where
-"seq_nop _ _ m m"
+inductive seq_nop :: "'sq \<Rightarrow> 'mstate \<Rightarrow> 'mstate \<Rightarrow> bool" where
+"seq_nop _ m m"
 
 locale Seq_Semantics = Seq_Semantics_Sig 
 begin
 
 print_context
 
-(* problem - this specifies next behavior for all base nodes
-   is that really what we want? it may actually be, i'm just not sure. *)
-(* another option is to just have this encapsulate descending into a base
-   node and handling "next" elsewhere, perhaps at the "elle" level... *)
-(* a third option is to only use "unhandled" cases *)
-(* another way to get at this: what should the hierarchy look like? *)
-(* hierarchy: can we worry about it later? *)
-inductive seq_rec_sem :: "'c \<Rightarrow> ('d, 'xb, 'xa) syn_seq \<Rightarrow> 'b \<Rightarrow> 'b \<Rightarrow>
-  childpath \<Rightarrow> ('bs, ('d, 'xb, 'xa) syn_seq, 'c) gensyn \<Rightarrow> ('a) gs_result \<Rightarrow> bool" where
-"seq_sem g s m m' \<Longrightarrow> seq_rec_sem g (LSeq s) m m' cp sk (GRPath (cp@[0]))"
+inductive x_sem_seq :: "('c, 'xp, 'xs) syn_seq \<Rightarrow> 'b \<Rightarrow> 'b \<Rightarrow>
+  childpath \<Rightarrow> ('c, 'xp, 'xs) syn_seq gensyn \<Rightarrow> ('a) gs_result \<Rightarrow> bool" where
+"seq_sem s m m' \<Longrightarrow> x_sem_seq (LSeq s xp) m m' cp g (GRPath (cp@[0]))"
 
 end
 
@@ -31,24 +24,24 @@ end
   ...
 *)
 
-locale Base_Next_Semantics = Gensyn_Semantics_Base_Sig 
+locale Base_Next_Semantics = Gensyn_Semantics_Sig
 begin
 
 print_context
 
-inductive base_sem_next ::
-    "'c \<Rightarrow> 'd \<Rightarrow> 'b \<Rightarrow> 'b \<Rightarrow> childpath \<Rightarrow>
-            ('d, 'e, 'c) gensyn \<Rightarrow>
+inductive x_sem_next ::
+    "'c \<Rightarrow> 'b \<Rightarrow> 'b \<Rightarrow> childpath \<Rightarrow>
+            ('c) gensyn \<Rightarrow>
                  ('a) gs_result \<Rightarrow> bool"
     where
-"base_sem g b m m' cp t GRUnhandled \<Longrightarrow>
+"x_sem x m m' cp t GRUnhandled \<Longrightarrow>
  gensyn_cp_next t cp = Some cp' \<Longrightarrow>
-  base_sem_next g b m m' cp t (GRPath cp')"
-| "base_sem g b m m' cp t GRUnhandled \<Longrightarrow>
+  x_sem_next x m m' cp t (GRPath cp')"
+| "x_sem x m m' cp t GRUnhandled \<Longrightarrow>
   gensyn_cp_next t cp = None \<Longrightarrow>
-  base_sem_next g b m m' cp t (GRDone)"
-| "base_sem g b m m' cp t res \<Longrightarrow>
-  base_sem_next g b m m' cp t res"
+  x_sem_next x m m' cp t (GRDone)"
+| "x_sem x m m' cp t res \<Longrightarrow>
+  x_sem_next x m m' cp t res"
 
 end
 
