Syntax/Syn_I.thy
@@ -1,12 +1,22 @@
-theory Syn_I imports "../Syntax_Utils"
+theory Syn_I imports "MiniPack"
 begin
 (* Syntax with instructions *)
 (* This serves as a template for what
 base-case syntax instatiations look like *)
 
+type_synonym ('d, 'xp, 'xs) syn_i = "('d, 'xp, 'xs) mpack"
 
-type_synonym ('i, 'xb, 'xa) syn_i =
-  "('xb + 'i + 'xa)"
+fun snd' :: "('a * 'b) \<Rightarrow> 'b" where
+"snd' (_, b) = b"
+
+
+(*
+definition LInst :: "'i \<Rightarrow> 'xp \<Rightarrow> ('i, 'xp, 'xs) syn_i" where
+"LInst x xp = (Inl x, xp)"
+*)
+(*
+type_synonym ('d, 'bp, 'ap, 'bs, 'as)  syn_i = "('d, 'bp, 'ap, 'bs, 'as) pack"
+type_synonym 'i dsyn_i = "'i dpack"
 
 (* there are other discriminator forms, see Alt_Sym.thy.
    i think this is the one we want... *)
@@ -23,5 +33,6 @@ definition LInst :: "'i \<Rightarrow> ('i, 'xb, 'xa) syn_i" where
 
 (* have a syn_i_dat definition to allow more annotations at the node?
    see seq e.g. *)
+*)
 
 end
