Syntax/Syn_Seq.thy
@@ -1,26 +1,25 @@
-theory Syn_Seq imports "../Syntax_Utils"
+theory Syn_Seq imports "../Syntax_Utils" "MiniPack"
 begin
 
-type_synonym ('sq, 'xb, 'xa) syn_seq =
-  "('xb + 'sq + 'xa)"
+type_synonym ('sq, 'xp, 'xs) syn_seq =
+  "('sq, 'xp, 'xs) mpack"
 
 type_synonym ('sq, 'xb, 'xa, 'o) syn_seq_disc =
-  "('xb * ('sq \<Rightarrow> 'o) * 'xa)"
+  "('sq, 'xb, 'xa, 'o) mp_disc"
 
+(*
 fun syn_seq_cases ::
-  "('sq, 'xb, 'xa) syn_seq \<Rightarrow> ('sq, 'xb \<Rightarrow> 'o, 'xa \<Rightarrow> 'o, 'o) syn_seq_disc \<Rightarrow> 'o" where
+  "('sq, 'xb, 'xa) syn_seq \<Rightarrow> 
+   ('sq, 'xb \<Rightarrow> 'o, 'xa \<Rightarrow> 'o, 'o) syn_seq_disc \<Rightarrow> 'o" where
   "syn_seq_cases s d = disc3 s d"
+*)
 
 (* may run into issues with phantom type variables here *)
-definition LSeq :: "'sq \<Rightarrow> ('sq, 'xb, 'xa) syn_seq" where
-    "LSeq x = snth2h x"
-
-
-type_synonym ('sq, 'xb, 'xa) dat_seq =
-  "('xb * 'sq * 'xa)"
+definition LSeq :: "'sq \<Rightarrow> 'xp \<Rightarrow> ('sq, 'xp, 'xs) syn_seq" where
+    "LSeq sq xp = mp_constr sq xp"
 
 (* scoping, used in Elle *)
-type_synonym ('sqb, 'sqa, 'xb, 'xa) syn_seq_scope =
-  "((nat list option, 'sqb, 'sqa) dat_seq, 'xb, 'xa) syn_seq"
+type_synonym ('xp1, 'xs1, 'xp2, 'xs2) syn_seq_scope =
+  "((nat list option, 'xp1, 'xs1) mpack, 'xp2, 'xs2) mpack"
 
 end
